x86/PseudoInstructions.v
@@ -1,0 +1,147 @@
+Require Import Coqlib Integers AST Memdata Maps.
+Require Import Asm Asmgen RealAsm.
+Require Import Errors.
+Require Import Memory.
+Import ListNotations.
+
+Local Open Scope error_monad_scope.
+Close Scope nat_scope.
+
+Definition linear_addr reg ofs :=
+  Addrmode (Some reg) None (inl ofs).
+
+Definition Plea := if Archi.ptr64 then Pleaq else Pleal.
+Definition Padd dst src z := Plea dst (linear_addr src z).
+Definition Psub dst src z := Padd dst src (- z).
+
+Definition Pstoreptr := if Archi.ptr64 then Pmovq_mr else Pmovl_mr.
+
+(* Pstoreptr (linear addr ) (RAX) eval_addrmode32 *)
+Definition transf_instr (i: instruction): list instruction :=
+  match i with
+  | Pallocframe sz ofs_ra ofs_link =>
+    let sz := align sz 8 - size_chunk Mptr in
+    let addr := linear_addr RSP (Ptrofs.unsigned ofs_link) in
+    [ Padd RAX RSP (size_chunk Mptr); Psub RSP RSP sz; Pstoreptr addr RAX]
+  | Pfreeframe fsz ofs_ra ofs_link =>
+    let sz := align fsz 8 - size_chunk Mptr in
+    [ Padd RSP RSP sz ]
+  | _ => [ i ]
+  end.
+
+Definition transf_code (c: code) : code :=
+  concat (map transf_instr c).
+
+Definition transf_function (f: function) : function :=
+  {|
+    fn_sig := fn_sig f;
+    fn_code := transf_code (fn_code f);
+    fn_stacksize := fn_stacksize f;
+    fn_ofs_link := fn_ofs_link f;
+  |}.
+
+Definition transf_fundef := AST.transf_fundef transf_function.
+
+Definition transf_program (p: Asm.program) : Asm.program :=
+  AST.transform_program transf_fundef p.
+
+(*
+Definition check_function (f: Asm.function) : bool :=
+  wf_asm_function_check f && AsmFacts.check_asm_code_no_rsp (fn_code f).
+
+Definition transf_check_function f :=
+  if check_function f then OK f
+  else Error (MSG "Precondition of pseudo instruction elimination fails" :: nil).
+
+Definition transf_check_fundef :=
+  AST.transf_partial_fundef (transf_check_function).
+
+Require Import Globalenvs.
+
+(* Definition has_main (p: program) := *)
+(*   let ge := Genv.globalenv p in *)
+(*   match Genv.find_symbol ge (prog_main p) with *)
+(*   | Some b => *)
+(*     match Genv.find_funct_ptr ge b with *)
+(*     | Some (Internal f) => true *)
+(*     | _ => false *)
+(*     end *)
+(*   | _ => false *)
+(*   end. *)
+
+Definition check_program p : res (Asm.program) :=
+  (* if has_main p *)
+  (* then *) AST.transform_partial_program transf_check_fundef p
+  (* else Error (msg "no main function in program") *).
+
+Theorem check_program_id:
+  forall p1 p2,
+    check_program p1 = OK p2 -> p1 = p2.
+Proof.
+  unfold check_program.
+  unfold transform_partial_program.
+  unfold transform_partial_program2.
+  intros. monadInv H. destruct p1. simpl in *. f_equal.
+  revert EQ.
+  unfold transf_check_fundef, transf_partial_fundef, transf_check_function.
+  revert x; induction prog_defs; simpl; intros; eauto. inv EQ; auto.
+  destr_in EQ.
+  repeat destr_in EQ; repeat destr_in Heqr; monadInv H0.
+  - f_equal. eauto.
+  - f_equal. eauto.
+  - f_equal; eauto. f_equal. f_equal. f_equal. destruct v; simpl. f_equal.
+  - f_equal. eauto.
+Qed.
+
+Definition match_check_prog (p: Asm.program) (tp: Asm.program) :=
+  Linking.match_program (fun _ f tf => transf_check_fundef f = OK tf) eq p tp (* /\ *)
+  (* exists (bmain : Values.block) (fmain : Asm.function), *)
+  (*   Globalenvs.Genv.find_symbol (Globalenvs.Genv.globalenv p) (prog_main p) = Some bmain /\ *)
+  (*   Globalenvs.Genv.find_funct_ptr (Globalenvs.Genv.globalenv p) bmain = Some (Internal fmain) *).
+
+Lemma check_program_match:
+  forall p tp, check_program p = OK tp -> match_check_prog p tp.
+Proof.
+  intros. unfold check_program in H. destr_in H.
+  eapply Linking.match_transform_partial_program; eauto.
+Qed.
+
+Theorem check_wf:
+  forall p tp,
+    match_check_prog p tp ->
+    RealAsm.wf_asm_prog (Globalenvs.Genv.globalenv p).
+Proof.
+  red.
+  intros.
+  destruct H as (A & B & C).
+  eapply Globalenvs.Genv.find_funct_ptr_prop with (P := fun f => match f with Internal f => _ f | _ => True end) in H0.
+  apply H0.
+  intros. edestruct list_forall2_in_left as (v2 & IN2 & P2); eauto.
+  inv P2. simpl in *. subst. inv H2. inv H4.
+  destr. simpl in H5. monadInv H5.
+  unfold transf_check_function in EQ. repeat destr_in EQ.
+  unfold check_function in Heqb0.
+  apply andb_true_iff in Heqb0; destruct Heqb0.
+  eapply wf_asm_function_check_correct; eauto.
+Qed.
+
+Theorem check_no_rsp:
+  forall p tp,
+    match_check_prog p tp ->
+    forall b f,
+      Globalenvs.Genv.find_funct_ptr (Globalenvs.Genv.globalenv p) b = Some (Internal f) ->
+      AsmFacts.check_asm_code_no_rsp (fn_code f) = true.
+Proof.
+  intros.
+  destruct H as (A & B & C).
+  eapply Globalenvs.Genv.find_funct_ptr_prop with (P := fun f => match f with Internal f => _ f | _ => True end) in H0.
+  pattern f.
+  apply H0.
+  simpl. intros. edestruct list_forall2_in_left as (v2 & IN2 & P2); eauto.
+  inv P2. simpl in *. subst. inv H2. inv H4.
+  destr. simpl in H5. monadInv H5.
+  unfold transf_check_function in EQ. repeat destr_in EQ.
+  unfold check_function in Heqb0.
+  apply andb_true_iff in Heqb0; destruct Heqb0; auto.
+Qed.
+*)
