x86/PseudoInstructionsproof.v
@@ -1,0 +1,548 @@
+Require Import Smallstep.
+Require Import Machregs.
+Require Import Asm.
+Require Import Integers.
+Require Import List.
+Require Import ZArith.
+Require Import Memtype.
+Require Import Memory.
+Require Import Archi.
+Require Import Coqlib.
+Require Import AST.
+Require Import Globalenvs.
+Require Import Events.
+Require Import Values.
+Require Import Conventions1.
+Require Import AsmFacts.
+Require Import RealAsm PseudoInstructions.
+Require Import RealAsmproof.
+Require Import AsmRegs.
+
+Definition match_prog (p: Asm.program) (tp: Asm.program) :=
+  Linking.match_program (fun _ f tf => tf = transf_fundef f) eq p tp.
+
+Lemma transf_program_match:
+  forall p tp, transf_program p = tp -> match_prog p tp.
+Proof.
+  intros. subst. eapply Linking.match_transform_program; eauto.
+Qed.
+
+Section PRESERVATION.
+
+  Variable prog tprog: Asm.program.
+  Hypothesis TRANSF: Linking.match_program (fun _ f1 f2 => f2 = transf_fundef f1) eq prog tprog.
+  Let ge := Genv.globalenv prog.
+  Let tge := Genv.globalenv tprog.
+
+  Lemma symbols_preserved:
+    forall (s: ident), Genv.find_symbol tge s = Genv.find_symbol ge s.
+  Proof (Genv.find_symbol_match TRANSF).
+
+  Lemma senv_preserved:
+    Senv.equiv ge tge.
+  Proof (Genv.senv_match TRANSF).
+
+(*  Lemma genv_next_preserved:
+    Genv.genv_next tge = Genv.genv_next ge.
+  Proof. apply senv_preserved. Qed. *)
+
+  Lemma functions_translated:
+    forall b f,
+      Genv.find_funct_ptr ge b = Some f ->
+      Genv.find_funct_ptr tge b = Some (transf_fundef f).
+  Proof. apply (Genv.find_funct_ptr_transf TRANSF). Qed.
+
+  Lemma functions_transl:
+    forall fb f,
+      Genv.find_funct_ptr ge fb = Some (Internal f) ->
+      Genv.find_funct_ptr tge fb = Some (Internal (transf_function f)).
+  Proof.
+    intros. apply functions_translated in H; eauto.
+  Qed.
+
+  Lemma public_preserved:
+    forall id : ident, Genv.public_symbol (Genv.globalenv tprog) id = Genv.public_symbol (Genv.globalenv prog) id.
+  Proof.
+    apply senv_preserved.
+  Qed.
+(* Does this matters?
+  Lemma transf_instr_size:
+    forall i,
+      instr_size i = code_size (transf_instr i).
+  Proof.
+    destruct i; simpl; try omega; rewrite Z.add_0_r.
+    apply instr_size_alloc; eauto.
+    apply instr_size_free; eauto.
+    apply instr_size_load_parent_pointer; eauto.
+  Qed.
+*)
+
+  Inductive code_at: Z -> code -> code -> Prop :=
+  | code_at_nil o c: code_at o c nil
+  | code_at_cons o c i c':
+      find_instr o c = Some i ->
+      code_at (o + instr_size i) c c' ->
+      code_at o c (i::c').
+
+  Lemma code_size_app:
+    forall c1 c2,
+      code_size (c1 ++ c2) = code_size c1 + code_size c2.
+  Proof.
+    induction c1; simpl; intros; eauto. rewrite IHc1. omega.
+  Qed.
+
+  Lemma code_at_app:
+    forall b a c, code_at (code_size a) (a ++ (b ++ c)) b.
+  Proof.
+    induction b; intros.
+    - constructor.
+    - constructor. 
+      replace (code_size a0) with (0 + code_size a0) by omega.
+      rewrite find_instr_app by omega. reflexivity.
+      replace (a0 ++ (a::b) ++ c) with ((a0 ++ a::nil) ++ b ++ c).
+      replace (code_size a0 + instr_size a) with (code_size (a0 ++ a::nil)).
+      apply IHb.
+      rewrite code_size_app. simpl. omega.
+      simpl. rewrite app_ass. simpl. reflexivity.
+  Qed.
+
+  Lemma code_at_next:
+    forall a i b, code_at (instr_size i) (i :: a ++ b) a.
+  Proof.
+    intros.
+    generalize (code_at_app a (i::nil) b). simpl. auto.
+  Qed.
+
+  Lemma code_at_shift:
+    forall i a c o,
+      code_at (o - code_size a) c i -> code_at o (a ++ c) i.
+  Proof.
+    induction i; simpl; intros b c o CA. constructor.
+    inv CA. constructor.
+    replace o with ((o - code_size b) + code_size b) by omega.
+    rewrite find_instr_app. auto. eapply find_instr_pos_positive; eauto.
+    apply IHi.
+    replace (o + instr_size a - code_size b) with (o - code_size b + instr_size a). auto. omega.
+  Qed.
+(*
+  Lemma find_instr_transl:
+    forall c o i,
+      find_instr o c = Some i ->
+      code_at o (transf_code c) (transf_instr i).
+  Proof.
+    induction c; simpl; intros; eauto. easy.
+    repeat destr_in H.
+    - unfold transf_code. simpl.
+      destruct transf_instr eqn:TI.
+      apply (f_equal code_size) in TI. rewrite <- transf_instr_size in TI. simpl in TI. generalize (instr_size_positive i); omega.
+      simpl. constructor. simpl. auto.
+      simpl. apply code_at_next.
+    - specialize (IHc _ _ H1).
+      unfold transf_code. simpl. fold (transf_code c).
+      eapply code_at_shift. rewrite <- transf_instr_size; auto.
+  Qed.
+*)
+  Definition id_instr (i: instruction) : bool :=
+    match i with
+    | Pallocframe _ _ _
+    | Pfreeframe _ _ _ => false
+    | _ => true
+    end.
+
+  Hypothesis WF: wf_asm_prog ge.
+  Hypothesis prog_no_rsp: asm_prog_no_rsp ge.
+
+  Lemma exec_instr_Plea:
+    forall ge f r a (rs: regset) m,
+      exec_instr ge f (Plea r a) rs m =
+      Next (nextinstr (rs # r <- (eval_addrmode ge a rs))) m.
+  Proof.
+    unfold Plea, eval_addrmode.
+    intros. destr.
+  Qed.
+
+  Lemma ptrofs_eq_unsigned: forall a b,
+      Ptrofs.unsigned a = Ptrofs.unsigned b -> a = b.
+  Proof.
+    intros.
+    rewrite <- (Ptrofs.repr_unsigned a).
+    rewrite <- (Ptrofs.repr_unsigned b).
+    rewrite H. reflexivity.
+  Qed.
+
+  Lemma eval_addrmode_offset_ptr:
+    forall (rs: regset) (r: ireg) z (RSPPTR: exists b o, rs r = Vptr b o),
+      eval_addrmode (Genv.globalenv tprog) (linear_addr r z) rs = Val.offset_ptr (rs r) (Ptrofs.repr z).
+  Proof.
+    unfold eval_addrmode. intros.
+    destr.
+    ++ unfold eval_addrmode64, linear_addr.
+       destruct (RSPPTR) as (bb & o & RSPPTR'). rewrite RSPPTR'. simpl. rewrite Heqb.
+       f_equal. rewrite Int64.add_zero_l. f_equal.
+       erewrite Ptrofs.agree64_of_int_eq. eauto. apply Ptrofs.agree64_repr; auto.
+    ++ unfold eval_addrmode32, linear_addr.
+       destruct (RSPPTR) as (bb & o & RSPPTR'). rewrite RSPPTR'. simpl. rewrite Heqb.
+       f_equal. rewrite Int.add_zero_l. f_equal.
+       erewrite Ptrofs.agree32_of_int_eq. eauto. apply Ptrofs.agree32_repr; auto.
+  Qed.
+
+  Lemma id_instr_transf:
+    forall i,
+      id_instr i = true ->
+      transf_instr i = i :: nil.
+  Proof.
+    destruct i; simpl; intros; congruence.
+  Qed.  
+
+  Lemma eval_addrmode64_senv_equiv:
+    forall (ge1 ge2: genv) (EQ: Senv.equiv ge1 ge2) a rs,
+      eval_addrmode64 ge1 a rs = eval_addrmode64 ge2 a rs.
+  Proof.
+    intros.
+    unfold eval_addrmode64.
+    destr. unfold Genv.symbol_address.
+    destruct const. auto. destruct p.
+    destruct EQ as (A & B & C). simpl in *. rewrite A. auto.
+  Qed.
+
+  Lemma eval_addrmode32_senv_equiv:
+    forall (ge1 ge2: genv) (EQ: Senv.equiv ge1 ge2) a rs,
+      eval_addrmode32 ge1 a rs = eval_addrmode32 ge2 a rs.
+  Proof.
+    intros.
+    unfold eval_addrmode32.
+    destr. unfold Genv.symbol_address.
+    destruct const. auto. destruct p.
+    destruct EQ as (A & B & C). simpl in *. rewrite A. auto.
+  Qed.
+
+  Lemma eval_addrmode_senv_equiv:
+    forall (ge1 ge2: genv) (EQ: Senv.equiv ge1 ge2) a rs,
+      eval_addrmode ge1 a rs = eval_addrmode ge2 a rs.
+  Proof.
+    unfold eval_addrmode.
+    intros.
+    destr; eauto using eval_addrmode64_senv_equiv, eval_addrmode32_senv_equiv.
+  Qed.
+
+  Lemma exec_load_senv_equiv:
+    forall (ge1 ge2: genv) (EQ: Senv.equiv ge1 ge2) chunk m a rs r,
+      exec_load ge1 chunk m a rs r =
+      exec_load ge2 chunk m a rs r .
+  Proof.
+    unfold exec_load.
+    intros; erewrite eval_addrmode_senv_equiv; eauto.
+  Qed.
+
+  Lemma exec_store_senv_equiv:
+    forall (ge1 ge2: genv) (EQ: Senv.equiv ge1 ge2) chunk m a rs r lr,
+      exec_store ge1 chunk m a rs r lr=
+      exec_store ge2 chunk m a rs r lr.
+  Proof.
+    unfold exec_store.
+    intros; erewrite eval_addrmode_senv_equiv; eauto.
+  Qed.
+
+  (* About label, maybe the reason why we need instr_size before *)
+  Lemma label_pos_app:
+    forall a b l o,
+      ~ In (Plabel l) a ->
+      label_pos l o (a ++ b) = label_pos l (o + code_size a) b.
+  Proof.
+    induction a; simpl; intros; eauto.
+    rewrite Z.add_0_r; auto.
+    destr. destruct a; simpl in Heqb0; try congruence. destr_in Heqb0.
+    rewrite IHa; auto. f_equal. unfold instr_size.  lia.
+  Qed.
+(*
+  Lemma label_pos_transf:
+    forall c l o,
+      label_pos l o c =
+      label_pos l o (transf_code c).
+  Proof.
+    induction c; simpl; intros; eauto.
+    unfold transf_code. simpl. fold (transf_code c).
+    destr.
+    - destruct a; simpl in Heqb; try congruence.
+      destr_in Heqb. subst. simpl. rewrite peq_true. reflexivity.
+    - rewrite label_pos_app.
+      rewrite <- transf_instr_size. auto.
+      intro IN.
+      destruct a; try now (simpl in *; unfold Padd, Psub, Plea in *; simpl in *; repeat destr_in IN; try intuition congruence).
+      simpl in *. destr_in Heqb.
+      simpl in *. unfold Padd, Psub, Plea in *. simpl in *. repeat destr_in IN. intuition congruence.
+      unfold Padd, Psub, Plea in *. repeat destr_in H. intuition congruence.
+      unfold Padd, Psub, Plea in *. repeat destr_in H.
+  Qed.
+
+  Lemma goto_label_senv_equiv:
+    forall f l rs m rs' m',
+      goto_label ge f l rs m = Next rs' m' ->
+      goto_label tge (transf_function f) l rs m = Next rs' m'.
+  Proof.
+    unfold goto_label.
+    intros.
+    simpl; rewrite <- label_pos_transf. destr.
+    destr.
+    destr_in H. inv H. erewrite functions_translated; eauto.
+  Qed.
+*)
+(*
+  Lemma goto_ofs_senv_equiv:
+    forall sz ofs rs m rs' m',
+      goto_ofs ge sz ofs rs m = Next rs' m' ->
+      goto_ofs tge sz ofs rs m = Next rs' m'.
+  Proof.
+    unfold goto_ofs.
+    intros.
+    destr.
+    destr_in H. inv H. erewrite functions_translated; eauto.
+  Qed.
+*)
+  Lemma functions_only_translated:
+    forall b,
+      Genv.find_funct_ptr ge b = None ->
+      Genv.find_funct_ptr tge b = None.
+  Proof.
+    destruct TRANSF as (A & B & C).
+    unfold Genv.find_funct_ptr, Genv.find_def.
+    unfold ge, tge, Genv.globalenv.
+    assert (REC:   forall b : block,
+               match NMap.get _ b (Genv.genv_defs (Genv.empty_genv Asm.fundef unit (prog_public prog))) with
+               | Some (Gfun f) => Some f
+               | Some (Gvar _) => None
+               | None => None
+               end = None ->
+               match NMap.get _ b (Genv.genv_defs (Genv.empty_genv Asm.fundef unit (prog_public tprog))) with
+               | Some (Gfun f) => Some f
+               | Some (Gvar _) => None
+               | None => None
+               end = None).
+    {
+      simpl. intros b. auto.
+    }
+(*    assert (NEXT: Genv.genv_next (Genv.empty_genv Asm.fundef unit (prog_public prog)) =
+                  Genv.genv_next (Genv.empty_genv Asm.fundef unit (prog_public tprog))).
+    {
+      reflexivity.
+    } *)
+    Admitted.
+(*
+    revert REC NEXT.
+    generalize (Genv.empty_genv Asm.fundef unit (prog_public prog)) (Genv.empty_genv Asm.fundef unit (prog_public tprog)).
+    revert A.
+    simpl.
+    unfold Asm.fundef.
+    generalize (@prog_defs (fundef function) unit prog) (@prog_defs (fundef function) unit tprog).
+    induction 1; simpl. eauto.
+    intros t t0 REC NEXT. apply IHA.
+    simpl. intro b. inv H. inv H1. auto.
+    rewrite ! Maps.PTree.gsspec.
+    rewrite NEXT. destruct (peq b (Genv.genv_next t0)). inv H3. congruence. auto. auto.
+    simpl. congruence.
+  Qed.
+  *)
+
+(*
+  Lemma goto_label_senv_equiv':
+    forall f l rs m,
+      goto_label ge f l rs m = Stuck ->
+      goto_label tge (transf_function f) l rs m = Stuck.
+  Proof.
+    unfold goto_label.
+    intros.
+    simpl; rewrite <- label_pos_transf. destr.
+    destr.
+    destr_in H. erewrite functions_only_translated; eauto.
+  Qed.
+
+  Lemma goto_ofs_senv_equiv':
+    forall sz ofs rs m,
+      goto_ofs ge sz ofs rs m = Stuck ->
+      goto_ofs tge sz ofs rs m = Stuck.
+  Proof.
+    unfold goto_ofs.
+    intros.
+    destr.
+    destr_in H. erewrite functions_only_translated; eauto.
+  Qed.
+
+  Lemma goto_label_eq:
+    forall f l rs m,
+      goto_label ge f l rs m =
+      goto_label tge (transf_function f) l rs m.
+  Proof.
+    intros.
+    destruct (goto_label ge f l rs m) eqn:GL.
+    symmetry; eapply goto_label_senv_equiv; eauto.
+    symmetry; eapply goto_label_senv_equiv'; eauto.
+  Qed.
+
+  Lemma goto_ofs_eq:
+    forall sz ofs rs m,
+      goto_ofs ge sz ofs rs m =
+      goto_ofs tge sz ofs rs m.
+  Proof.
+    intros.
+    destruct (goto_ofs ge sz ofs rs m) eqn:GL.
+    symmetry; eapply goto_ofs_senv_equiv; eauto.
+    symmetry; eapply goto_ofs_senv_equiv'; eauto.
+  Qed.
+
+  Lemma eval_ros_eq:
+    forall ros rs,
+      eval_ros ge ros rs = eval_ros tge ros rs.
+  Proof.
+    unfold eval_ros.
+    intros. destr.
+    unfold Genv.symbol_address.
+    destruct senv_preserved as (A & B & C & D). simpl in *; rewrite B. auto.
+  Qed.
+  *)
+  Lemma exec_instr_senv_equiv:
+    forall f i rs m (ID : id_instr i = true),
+      exec_instr ge f i rs m = exec_instr tge (transf_function f) i rs m.
+  Proof.
+    generalize senv_preserved as EQ.
+    destruct i; simpl; intros; eauto using exec_load_senv_equiv, exec_store_senv_equiv;
+      inversion EQ as (A & B & C); simpl in *.
+    -
+    unfold Genv.symbol_address. rewrite A. auto.
+    -
+    erewrite eval_addrmode32_senv_equiv; eauto.
+    -
+    erewrite eval_addrmode64_senv_equiv; eauto.
+    -
+    admit.
+(*    eapply goto_label_eq; eauto. *)
+    -
+      unfold Genv.find_funct. unfold Genv.symbol_address. rewrite A.
+      repeat destr.
+      destr_in Heqo. exploit functions_translated; eauto. intro. congruence.
+      destr_in Heqo. exploit functions_only_translated; eauto. intro. congruence.
+    -
+      unfold Genv.find_funct. repeat destr.
+      repeat destr_in Heqo. exploit functions_translated; eauto. intro. congruence.
+      repeat destr_in Heqo. exploit functions_only_translated; eauto. intro. congruence.
+    -
+      destr. destr. admit. (*label*)
+    -
+      destr. destr. destr. destr. admit. (* eapply goto_label_eq; eauto. *)
+    -
+    destr. destr. admit.  (*eapply goto_label_eq; eauto. *)
+    -
+    destr. f_equal. f_equal. f_equal.  unfold Genv.symbol_address. rewrite A. auto.
+(*
+    eapply goto_ofs_eq; eauto.
+    destr. destr. eapply goto_ofs_eq; eauto.
+    destr. destr. destr. destr. eapply goto_ofs_eq; eauto.
+    destr. destr. eapply goto_ofs_eq; eauto.
+*)
+ Admitted.
+
+  Lemma pseudo_instructions_step:
+    forall s1 t s2
+           (STEP : step (Genv.globalenv prog) s1 t s2)
+           (INV: real_asm_inv s1),
+      plus step (Genv.globalenv tprog) s1 t s2.
+  Proof.
+    intros s1 t s2 STEP INV.
+    inv STEP.
+    - exploit functions_transl. eauto. intros FFP.
+      exploit find_instr_transl; eauto. intro CA.
+      destruct (id_instr i) eqn:ID; [| destruct i; simpl in ID; try congruence].
+      + pose proof (id_instr_transf _ ID) as NORMAL.
+        rewrite NORMAL in CA. inv CA.  inv H8. eapply plus_one.
+        econstructor. eauto. eapply FFP. eauto.
+        erewrite <- exec_instr_senv_equiv; eauto.
+      + subst; simpl in *. inv H2. inv CA. inv H7. inv H9.
+        eapply plus_two.
+        econstructor. eauto. eapply FFP. eauto.
+        unfold Padd. apply exec_instr_Plea.
+        econstructor. rewrite Asmgenproof0.nextinstr_pc. repeat rewrite Pregmap.gso by congruence.
+        rewrite H. simpl. eauto.
+        eauto. erewrite wf_asm_pc_repr'; eauto.
+        erewrite (instr_size_alloc sz pubrange ofs_ra (align sz 8 - size_chunk Mptr)
+                                   (size_chunk Mptr)).
+        generalize (instr_size_positive (Psub RSP RSP (align sz 8 - size_chunk Mptr))).
+        unfold Padd.
+        generalize (instr_size_positive (Plea RAX (linear_addr RSP (size_chunk Mptr)))).
+        omega.
+        unfold Psub, Padd. rewrite exec_instr_Plea. f_equal.
+        apply Axioms.extensionality. intro r.
+        destruct (preg_eq r PC).
+        * subst. simpl_regs. rewrite H. simpl. f_equal.
+          generalize (wf_asm_pc_repr' _ (WF _ _ H0) _ _ H1). intro REPR.
+          apply ptrofs_eq_unsigned. 
+          rewrite Ptrofs.add_assoc. rewrite (Ptrofs.add_unsigned (Ptrofs.repr _)).
+          erewrite Ptrofs.unsigned_repr by apply instr_size_repr.
+          erewrite Ptrofs.unsigned_repr by apply instr_size_repr.
+          repeat rewrite ! REPR.
+          erewrite instr_size_alloc. unfold Psub, Padd; eauto.
+          generalize (instr_size_positive (Pallocframe sz pubrange ofs_ra)); omega.
+          setoid_rewrite <- (instr_size_alloc sz pubrange ofs_ra).
+          generalize (instr_size_positive (Pallocframe sz pubrange ofs_ra)); omega.
+        * simpl_regs. regs_eq. repeat rewrite Asmgenproof0.nextinstr_inv by auto.
+          regs_eq. auto.
+          apply eval_addrmode_offset_ptr. inv INV. edestruct RSPPTR as ( bb & oo & EQ & _); eauto.
+          rewrite eval_addrmode_offset_ptr; simpl_regs.
+          2: inv INV; edestruct RSPPTR as ( bb & oo & EQ & _); eauto.
+          f_equal.
+          unfold Ptrofs.neg. f_equal. f_equal.
+          eapply wf_allocframe_repr; eauto.
+        * traceEq.
+      + subst; simpl in *. inv H2. inv CA. inv H7.
+        eapply plus_one.
+        econstructor. eauto. eapply FFP. eauto.
+        unfold Padd. rewrite exec_instr_Plea.
+        f_equal. apply Axioms.extensionality. intro r.
+        erewrite (instr_size_free). unfold Padd.
+        regs_eq. auto.
+        rewrite eval_addrmode_offset_ptr.
+        2: inv INV; edestruct RSPPTR as ( bb & oo & EQ & _); eauto.
+        f_equal.
+        eapply wf_freeframe_repr; eauto.
+      + subst; simpl in *. inv H2. inv CA. inv H7.
+        eapply plus_one.
+        econstructor. eauto. eapply FFP. eauto.
+        unfold Padd. rewrite exec_instr_Plea.
+        f_equal. apply Axioms.extensionality. intro r.
+        setoid_rewrite Pregmap.gsspec. destr. repeat rewrite Pregmap.gso by congruence.
+        (* setoid_rewrite <- instr_size_load_parent_pointer. eauto. *)
+        setoid_rewrite Pregmap.gsspec. destr.
+        apply eval_addrmode_offset_ptr.
+        inv INV. edestruct RSPPTR as ( bb & oo & EQ & _); eauto.
+    - exploit functions_transl. eauto. intros FFP.
+      exploit find_instr_transl; eauto. intro CA.
+      apply plus_one.
+      inv CA. inv H9.
+      eapply exec_step_builtin; eauto.
+      eapply eval_builtin_args_preserved. apply senv_preserved. eauto.
+      eapply external_call_symbols_preserved. apply senv_preserved. eauto.
+    - exploit functions_translated. eauto. intros FFP.
+      apply plus_one.
+      eapply exec_step_external; eauto.
+      eapply external_call_symbols_preserved. apply senv_preserved. eauto.
+  Qed.
+  
+  Theorem pseudo_instructions_correct rs:
+    forward_simulation (RealAsm.semantics prog rs) (RealAsm.semantics tprog rs).
+  Proof.
+    eapply forward_simulation_plus with (match_states := fun s1 s2 : Asm.state => s1 = s2 /\ real_asm_inv prog s1).
+    - simpl. apply public_preserved.
+    - simpl; intros s1 IS1. inversion IS1.
+      eapply Genv.init_mem_transf in H; eauto. eexists; split;[|split]; eauto.
+      econstructor. eauto.
+      inv H0. unfold rs0. unfold ge0.
+      rewrite <- symbols_preserved in H1.
+      erewrite <- (Linking.match_program_main) in H1 by eauto.
+      econstructor; eauto.
+      eapply real_initial_inv; eauto.
+    - simpl; intros s1 s2 r (MS & INV) FS. subst. auto.
+    - simpl. intros s1 t s2 STEP s1' (MS & INV). subst.
+      eexists; split; [|split]; eauto.
+      eapply pseudo_instructions_step; eauto.
+      eapply real_asm_inv_inv; eauto.
+  Qed.
+
+End WITHMEMORYMODEL.
